theory/Static_Semantics.thy
@@ -148,5 +148,30 @@ fun value_to_abstract_value :: "val \<Rightarrow> abstract_value" ("|_|" [0]61) 
   "|VClsr p \<rho>| = ^p"
 
 
+inductive static_reachable :: "exp \<Rightarrow> exp \<Rightarrow> bool"  where
+  Refl : "
+    static_reachable e e
+  " | 
+  Let_Spawn_Child: "
+    static_reachable e\<^sub>c e \<Longrightarrow>
+    static_reachable (Let x (Spwn e\<^sub>c) e\<^sub>n) e
+  " |
+  let_case_left: "
+    static_reachable e\<^sub>l e \<Longrightarrow>
+    static_reachable (Let x (Case x\<^sub>s x\<^sub>l e\<^sub>l x\<^sub>r e\<^sub>r) e\<^sub>n) e
+  " |
+  let_case_right: "
+    static_reachable e\<^sub>r e \<Longrightarrow>
+    static_reachable (Let x (Case x\<^sub>s x\<^sub>l e\<^sub>l x\<^sub>r e\<^sub>r) e\<^sub>n) e
+  " |
+  Let_Abs_Body: "
+    static_reachable e\<^sub>b e \<Longrightarrow>
+    static_reachable (Let x (Prim (Abs f x\<^sub>p e\<^sub>b)) e\<^sub>n) e
+  " | 
+  Let: "
+    static_reachable e\<^sub>n e \<Longrightarrow>
+    static_reachable (Let x b e\<^sub>n) e
+  "
+
 
 end
